reenable Impl.delete_avl
benchs soon

Impl.AVL.fst
@@ -383,7 +383,6 @@ let rec insert_avl (#a: Type)
   )
 #pop-options
 
-(*)
 #push-options "--fuel 1 --ifuel 1 --z3rlimit 100"
 let rec remove_leftmost_avl (#a: Type0) (cmp:cmp a) (ptr: t a)
   : Steel (t a & a)
@@ -398,8 +397,7 @@ let rec remove_leftmost_avl (#a: Type0) (cmp:cmp a) (ptr: t a)
     v_linked_tree (fst r) h1
     == fst (Spec.remove_leftmost_avl
       (convert cmp) (v_linked_tree ptr h0)) /\
-    snd r == snd (Spec.remove_leftmos
-t_avl
+    snd r == snd (Spec.remove_leftmost_avl
       (convert cmp) (v_linked_tree ptr h0)) /\
     Spec.size_of_tree (v_linked_tree (fst r) h1)
     == Spec.size_of_tree (v_linked_tree ptr h0) - 1 /\
@@ -411,19 +409,30 @@ t_avl
     let data = get_data node in
     elim_linked_tree_leaf (get_left node);
     free (get_size node);
+    free (get_height node);
     free ptr;
     return (get_right node, data)
   ) else (
     (**) not_null_is_node (get_left node);
     let r0 = remove_leftmost_avl cmp (get_left node) in
-    let old_size = read (get_size node) in
-    write (get_size node) (U.sub old_size one);
-    let new_node = mk_node (get_data node)
-      (fst r0) (get_right node) (get_size node) in
-    write ptr new_node;
-    (**) pack_tree ptr
-      (fst r0) (get_right node) (get_size node);
-    let new_ptr = rebalance_avl ptr in
+    let new_ptr = merge_tree_no_alloc
+      (get_data node) (fst r0) (get_right node)
+      (get_size node) (get_height node)
+      ptr in
+   // let old_size = read (get_size node) in
+   // write (get_size node) (U.sub old_size one);
+   // let height_right = hot_wdh (get_right node) in
+   // let height_new_left = hot_wdh (fst r0) in
+   // let new_height = U.add (umax height_right height_new_left) one in
+   // write (get_height node) new_height;
+   // let new_node = mk_node (get_data node)
+   //   (fst r0) (get_right node)
+   //   (get_size node) (get_height node) in
+   // write ptr new_node;
+   // (**) pack_tree ptr
+   //   (fst r0) (get_right node)
+   //   (get_size node) (get_height node);
+    let new_ptr = rebalance_avl cmp new_ptr in
     return (new_ptr, snd r0)
   )
 #pop-options
@@ -431,8 +440,10 @@ t_avl
 let cdata = Spec.cdata
 let cleft = Spec.cleft
 let cright = Spec.cright
+let csize = Spec.csize
+let cheight = Spec.cheight
 
-#push-options "--fuel 1 --ifuel 1 --z3rlimit 100"
+#push-options "--fuel 1 --ifuel 1 --z3rlimit 50"
 //#push-options "--fuel 1 --ifuel 1"
 let delete_avl_aux0 (#a: Type0)
   (cmp:cmp a) (ptr: t a) (data_to_rm: a)
@@ -447,148 +458,217 @@ let delete_avl_aux0 (#a: Type0)
     Spec.Node? (v_linked_tree ptr h0) /\
     Spec.is_avl (convert cmp) (v_linked_tree ptr h0) /\
     (convert cmp) (Spec.cdata (v_linked_tree ptr h0)) data_to_rm = 0 /\
-    (v_linked_tree ptr' h1
-    == Spec.delete_avl_aux0_wo_refinement
-      (convert cmp) (v_linked_tree ptr h0) data_to_rm) /\
-    Spec.size_of_tree (v_linked_tree ptr' h1)
-    == Spec.size_of_tree (v_linked_tree ptr h0) - 1)
+    v_linked_tree ptr' h1
+    == Spec.delete_avl_aux0
+      (convert cmp) (v_linked_tree ptr h0) data_to_rm)
   =
-  let h00 = get () in
   (**) node_is_not_null ptr;
   (**) let node = unpack_tree ptr in
-  if is_null_t (get_left node) && is_null_t (get_right node) then (
-    elim_linked_tree_leaf (get_left node);
-    free (get_size node);
-    free ptr;
-    return (get_right node)
-  ) else if is_null_t (get_right node) then (
+  if is_null_t (get_right node) then (
     elim_linked_tree_leaf (get_right node);
     free (get_size node);
+    free (get_height node);
     free ptr;
     return (get_left node)
   ) else if is_null_t (get_left node) then (
     elim_linked_tree_leaf (get_left node);
     free (get_size node);
+    free (get_height node);
     free ptr;
     return (get_right node)
   ) else (
-    let right_node = unpack_tree (get_right node) in
-    if is_null_t (get_left right_node) then (
-      let y = get_data right_node in
-      elim_linked_tree_leaf (get_left right_node);
-      free (get_size right_node);
-      free (get_right node);
-      let sz = read (get_size node) in
-      write (get_size node) (U.sub sz one);
-      let new_node = mk_node
-        y (get_left node) (get_right right_node) (get_size node) in
-      write ptr new_node;
-      pack_tree ptr
-        (get_left node) (get_right right_node) (get_size node);
-      return ptr
-    ) else (
-      pack_tree (get_right node)
-        (get_left right_node) (get_right right_node)
-        (get_size right_node);
-      let h0 = get () in
-      let result_spec = hide (Spec.remove_leftmost_avl
-        (convert cmp) (v_linked_tree (get_right node) h0)) in
-      let result = remove_leftmost_avl cmp (get_right node) in
-      assert (snd result == snd (reveal result_spec));
-      let sz = read (get_size node) in
-      write (get_size node) (U.sub sz one);
-      let h1 = get () in
-      assert (
-       Spec.size_of_tree (v_linked_tree (fst result) h1)
-       ==
-       Spec.size_of_tree (v_linked_tree (get_right node) h0) - 1);
-      assert (U.v (sel (get_size node) h0)
-      == Spec.size_of_tree (v_linked_tree (get_left node) h0)
-       + Spec.size_of_tree (v_linked_tree (get_right node) h0)
-       + 1);
-      assert (U.v (sel (get_size node) h0)
-      == U.v (sel (get_size node) h1) + 1);
-
-      let new_node = mk_node (snd result)
-        (get_left node) (fst result) (get_size node) in
-      write ptr new_node;
-      let h = get () in
-      assert (U.v (sel (get_size node) h)
-      == Spec.size_of_tree (v_linked_tree (get_left node) h)
-       + Spec.size_of_tree (v_linked_tree (fst result) h)
-       + 1);
-      pack_tree ptr
-        (get_left node) (fst result) (get_size node);
-      let orig = hide (v_linked_tree ptr h00) in
-      let result_spec = hide (Spec.delete_avl_aux0_wo_refinement
-        (convert cmp) (reveal orig) data_to_rm) in
-      let h = get () in
-      let result = hide (v_linked_tree ptr h) in
-      //assert (cdata (reveal result) == cdata (reveal result_spec));
-      //assert (cleft (reveal result) == cleft (reveal result_spec));
-      //assert (cright (reveal result) == cright (reveal result_spec));
-      return ptr
-    )
+    not_null_is_node (get_right node);
+    let r0 = remove_leftmost_avl cmp (get_right node) in
+    let new_ptr = merge_tree_no_alloc (snd r0)
+      (get_left node) (fst r0)
+      (get_size node) (get_height node)
+      ptr in
+    let new_ptr = rebalance_avl cmp new_ptr in
+    return new_ptr
   )
 #pop-options
 
-#push-options "--fuel 1 --ifuel 1"
-let delete_avl_aux1 (#a: Type0)
-  (cmp:cmp a) (ptr: t a) (data_to_rm: a)
-  : Steel (t a)
-  (linked_tree ptr)
-  (fun ptr' -> linked_tree ptr')
-  (requires fun h0 ->
-    Spec.Node? (v_linked_tree ptr h0) /\
-    Spec.is_avl (convert cmp) (v_linked_tree ptr h0) /\
-    (convert cmp) (Spec.cdata (v_linked_tree ptr h0)) data_to_rm = 0)
-  (ensures fun h0 ptr' h1 ->
-    Spec.Node? (v_linked_tree ptr h0) /\
-    Spec.is_avl (convert cmp) (v_linked_tree ptr h0) /\
-    (convert cmp) (Spec.cdata (v_linked_tree ptr h0)) data_to_rm = 0 /\
-    (v_linked_tree ptr' h1
-    == Spec.delete_avl_aux1
-      (convert cmp) (v_linked_tree ptr h0) data_to_rm) /\
-    Spec.is_avl (convert cmp) (v_linked_tree ptr' h1) /\
-    Spec.size_of_tree (v_linked_tree ptr' h1)
-    == Spec.size_of_tree (v_linked_tree ptr h0) - 1)
-  =
-  let h0 = get () in
-  assert (Spec.is_avl (convert cmp) (
-    Spec.delete_avl_aux1
-      (convert cmp) (v_linked_tree ptr h0) data_to_rm)
-  );
-  let ptr = delete_avl_aux0 cmp ptr data_to_rm in
-  rebalance_avl ptr
-#pop-options
+//#push-options "--fuel 1 --ifuel 1"
+//let delete_avl_aux1 (#a: Type0)
+//  (cmp:cmp a) (ptr: t a) (data_to_rm: a)
+//  : Steel (t a)
+//  (linked_tree ptr)
+//  (fun ptr' -> linked_tree ptr')
+//  (requires fun h0 ->
+//    Spec.Node? (v_linked_tree ptr h0) /\
+//    Spec.is_avl (convert cmp) (v_linked_tree ptr h0) /\
+//    (convert cmp) (Spec.cdata (v_linked_tree ptr h0)) data_to_rm = 0)
+//  (ensures fun h0 ptr' h1 ->
+//    Spec.Node? (v_linked_tree ptr h0) /\
+//    Spec.is_avl (convert cmp) (v_linked_tree ptr h0) /\
+//    (convert cmp) (Spec.cdata (v_linked_tree ptr h0)) data_to_rm = 0 /\
+//    (v_linked_tree ptr' h1
+//    == Spec.delete_avl_aux1
+//      (convert cmp) (v_linked_tree ptr h0) data_to_rm) /\
+//    Spec.is_avl (convert cmp) (v_linked_tree ptr' h1) /\
+//    Spec.size_of_tree (v_linked_tree ptr' h1)
+//    == Spec.size_of_tree (v_linked_tree ptr h0) - 1)
+//  =
+//  let h0 = get () in
+//  assert (Spec.is_avl (convert cmp) (
+//    Spec.delete_avl_aux1
+//      (convert cmp) (v_linked_tree ptr h0) data_to_rm)
+//  );
+//  let ptr = delete_avl_aux0 cmp ptr data_to_rm in
+//  rebalance_avl ptr
+//#pop-options
 
 let u_of_bool (b:bool) : x:U.t{U.v x = Spec.int_of_bool b}
 = match b with
 | true -> one
 | false -> zero
 
-#push-options "--fuel 1 --ifuel 1"
-inline_for_extraction noextract
-let dincr
-  (b: bool)
-  (ptr: ref U.t)
-  : Steel unit
-  (vptr ptr) (fun _ -> vptr ptr)
-  (requires fun h0 ->
-    U.gt (sel ptr h0) zero)
-  (ensures fun h0 _ h1 ->
-    (let old_value = sel ptr h0 in
-    U.gt (sel ptr h0) zero /\
-    sel ptr h1 = U.sub old_value (u_of_bool b)))
+//#push-options "--fuel 1 --ifuel 1"
+//inline_for_extraction noextract
+//let dincr
+//  (b: bool)
+//  (ptr: ref U.t)
+//  : Steel unit
+//  (vptr ptr) (fun _ -> vptr ptr)
+//  (requires fun h0 ->
+//    U.gt (sel ptr h0) zero)
+//  (ensures fun h0 _ h1 ->
+//    (let old_value = sel ptr h0 in
+//    U.gt (sel ptr h0) zero /\
+//    sel ptr h1 = U.sub old_value (u_of_bool b)))
+//  =
+//  if b then (
+//    let old_value = read ptr in
+//    write ptr (U.sub old_value one);
+//    return ()
+//  ) else (
+//    return ()
+//  )
+//#pop-options
+
+let delete_lemma (#a: Type0)
+  (cmp:Spec.cmp a) (t: Spec.avl a cmp) (data_to_rm: a)
+  : Lemma
+  (Spec.height_of_tree (Spec.delete_avl cmp t data_to_rm)
+  <= Spec.height_of_tree t)
   =
-  if b then (
-    let old_value = read ptr in
-    write ptr (U.sub old_value one);
-    return ()
+  Spec.delete_avl_aux_avl cmp t data_to_rm
+
+#push-options "--fuel 1 --ifuel 1 --z3rlimit 100"
+let rec delete_avl (#a: Type0)
+  (cmp:cmp a) (ptr: t a) (data_to_rm: a)
+  : Steel (t a) (linked_tree ptr) (fun ptr' -> linked_tree ptr')
+  (requires fun h0 ->
+    Spec.is_avl (convert cmp) (v_linked_tree ptr h0))
+  (ensures fun h0 ptr' h1 ->
+    Spec.is_avl (convert cmp) (v_linked_tree ptr h0) /\
+    Spec.delete_avl (convert cmp) (v_linked_tree ptr h0) data_to_rm
+    == v_linked_tree ptr' h1)
+    //Spec.height_of_tree (v_linked_tree ptr' h1)
+    //<= Spec.height_of_tree (v_linked_tree ptr h0))
+  =
+  //let h0 = get () in
+  //let t = hide (v_linked_tree ptr h0) in
+  //let t_s = hide (Spec.size_of_tree (reveal t)) in
+  //let t_h = hide (Spec.height_of_tree (reveal t)) in
+  //assert (t_s <= c);
+  //assert (t_h <= c);
+  if is_null_t #a ptr then (
+    (**) null_is_leaf ptr;
+    return ptr
   ) else (
-    return ()
+    (**) let node = unpack_tree ptr in
+    let delta = cmp data_to_rm (get_data node) in
+  if I.eq delta szero then (
+    pack_tree ptr
+      (get_left node) (get_right node)
+      (get_size node) (get_height node);
+    let ptr = delete_avl_aux0 cmp ptr data_to_rm in
+    return ptr
+  ) else if I.lt delta szero then (
+    let h0 = get () in
+    let new_left = delete_avl cmp (get_left node) data_to_rm in
+    let h1 = get () in
+    assert (v_linked_tree new_left h1
+    == Spec.delete_avl (convert cmp)
+      (v_linked_tree (get_left node) h0) data_to_rm);
+    delete_lemma (convert cmp)
+      (v_linked_tree (get_left node) h0) data_to_rm;
+    assert (Spec.height_of_tree (v_linked_tree new_left h1)
+    <= Spec.height_of_tree (v_linked_tree (get_left node) h0));
+    let new_ptr = merge_tree_no_alloc
+      (get_data node) new_left (get_right node)
+      (get_size node) (get_height node)
+      ptr in
+    let new_ptr = rebalance_avl cmp new_ptr in
+    return new_ptr
+  ) else (
+    let h0 = get () in
+    let new_right = delete_avl cmp (get_right node) data_to_rm in
+    let h1 = get () in
+    assert (v_linked_tree new_right h1
+    == Spec.delete_avl (convert cmp)
+      (v_linked_tree (get_right node) h0) data_to_rm);
+    delete_lemma (convert cmp)
+      (v_linked_tree (get_right node) h0) data_to_rm;
+    assert (Spec.height_of_tree (v_linked_tree new_right h1)
+    <= Spec.height_of_tree (v_linked_tree (get_right node) h0));
+    let new_ptr = merge_tree_no_alloc
+      (get_data node) (get_left node) new_right
+      (get_size node) (get_height node)
+      ptr in
+    let new_ptr = rebalance_avl cmp new_ptr in
+    return new_ptr
+  )
+  )
+
+(*)
+ let size_old_left = sot_wds (get_left node) in
+      let height_old_left = hot_wdh (get_left node) in
+      let size_new_left = sot_wds new_left in
+      let size_right = sot_wds (get_right node) in
+      let new_size = U.add (U.add size_new_left size_right) one in
+      write (get_size node) new_size;
+      let height_new_left = hot_wdh new_left in
+      let height_right = hot_wdh (get_right node) in
+      let new_height = U.add (umax height_new_left height_right) one in
+      write (get_height node) new_height;
+      assert (U.v size_new_left <= U.v size_old_left);
+      assert (U.v height_new_left <= U.v height_old_left);
+      let new_node = mk_node (get_data node)
+        new_left (get_right node)
+        (get_size node) (get_height node) in
+      write ptr new_node;
+
+
+    if I.gt delta szero then (
+      let h0 = get () in
+      let result = delete_avl_aux cmp (get_right node) data_to_rm in
+      dincr (snd result) (get_size node);
+      let h1 = get () in
+      assert (
+      U.v (sel (get_size node) h1)
+      ==
+      U.v (sel (get_size node) h0)
+      - (Spec.int_of_bool (snd result))
+      );
+      let new_node = mk_node (get_data node)
+        (get_left node) (fst result) (get_size node) in
+      write ptr new_node;
+      pack_tree ptr
+        (get_left node) (fst result) (get_size node);
+      let ptr = rebalance_avl ptr in
+      return (ptr, snd result)
+    ) else (
+      pack_tree ptr
+        (get_left node) (get_right node) (get_size node);
+      let ptr = delete_avl_aux1 cmp ptr data_to_rm in
+      return (ptr, true)
+    )
   )
 #pop-options
+
+
 
 
 #push-options "--fuel 1 --ifuel 1 --z3rlimit 100"
